isabelle/invariant.thy
@@ -166,8 +166,7 @@ lemma splice_app2:
   "length la = length lb \<Longrightarrow>
    splice (la @ [a]) (lb @ [b]) = ((splice la lb) @ [a]) @ [b]"
   apply(simp add: splice_appr) (* cong @[b] *)
-  apply(erule splice_appl)
-  done
+  by (erule splice_appl)
 
 lemma splice2:
   "\<lbrakk>drop n Qs = y # bs; drop n Ps = a # ls\<rbrakk>
@@ -183,22 +182,6 @@ lemma splice_set:
   "set (splice la lb) = set (la @ lb)"
   by (simp add: set_shuffles)
 
-lemma test2:
-  "\<And>tl p pp n y bs.
-       \<lbrakk>set Ps \<inter> set Qs = {}; length Qs \<le> length Ps; List tl pp (drop n Ps);
-        n \<le> length Qs; Path tl p (splice (take n Ps) (take n Qs)) pp;
-        drop n Qs = y # bs; List tl (tl y) bs; 0 < n \<or> pp \<noteq> p\<rbrakk>
-       \<Longrightarrow> List ((tl(y := tl (addr pp)))(pp \<rightarrow> Ref y)) (tl (addr pp))
-            (drop (Suc n) Ps)"
-  apply(cases Ps;clarsimp)
-  apply(subgoal_tac "List tl (tl (addr pp)) (drop (Suc n) (a # list))")
-  using notin_List_update
-   apply(smt List_hd_not_in_tl disjoint_iff drop_Suc in_set_dropD list.sel list.set_intros)
-  apply(subgoal_tac "n \<noteq> Suc (length list)")
-   apply(smt (verit) Cons_nth_drop_Suc List_def Path.simps(2) addr.simps le_neq_implies_less le_trans length_Cons)
-  apply(auto) (* n < length Qs \<le> Suc(length list) *)
-  done
-
 (* interleaves two lists. size invars always hold, p not modified *)
 lemma "VARS tl p q pp qq
   { List tl p Ps \<and> List tl q Qs
@@ -209,66 +192,66 @@ lemma "VARS tl p q pp qq
         set Ps \<inter> set Qs = {} \<and> size Qs \<le> size Ps \<and>
        (\<exists>n. List tl pp (drop n Ps) \<and> List tl q (drop n Qs) \<and>
          (n \<le> size Qs) \<and>
-        ((n = 0 \<and> pp = p) \<or>
-         Path tl p (splice (take n Ps) (take n Qs)) pp \<and>
+        (Path tl p (splice (take n Ps) (take n Qs)) pp \<and>
          List tl pp (drop n Ps)))
   }
   DO qq := q^.tl; q^.tl := pp^.tl; pp^.tl := q; pp := q^.tl; q := qq OD
   { List tl p (splice Ps Qs) }"
   apply(vcg)
-    apply(fastforce)
-   defer
+    apply(clarsimp)
+    apply(rule_tac x=0 in exI)
+    apply(simp)
    apply(clarsimp)
-   apply(case_tac "Qs = [] \<and> pp = p";clarsimp)
-  using splice1 List_app
-   apply(smt (verit) List_def List_distinct Path.simps(2) neq_dP)
-  apply(clarsimp)
-  apply(subgoal_tac "((tl(y := tl (addr pp)))(pp \<rightarrow> Ref y)) y = tl (addr pp)")
-   defer
-   apply(metis List_Ref List_conv_islist_list List_def Path.simps(1) addr.simps disjoint_iff drop_eq_Nil2 fun_upd_other fun_upd_same inf.bounded_iff inf.order_iff inf_left_idem list.set_intros(1) not_Null_eq set_drop_subset)
-  apply(simp)
-  apply(thin_tac "((tl(y := tl (addr pp)))(pp \<rightarrow> Ref y)) y = tl (addr pp)")
-  apply(rule_tac x="Suc n" in exI)
-  apply(case_tac "n = 0 \<and> pp = p";clarsimp)
+   apply(rule_tac x="Suc n" in exI)
+   apply(subgoal_tac "((tl(y := tl (addr pp)))(pp \<rightarrow> Ref y)) y = tl (addr pp)")
+    prefer 2
+    apply(metis List_Ref List_conv_islist_list List_def Path.simps(1) addr.simps disjoint_iff drop_eq_Nil2 fun_upd_other fun_upd_same inf.bounded_iff inf.order_iff inf_left_idem list.set_intros(1) not_Null_eq set_drop_subset)
+   apply(clarsimp)
    apply(rule conjI)
-    apply(smt (verit) List_def List_distinct Path.simps(2) Suc_le_length_iff addr.simps distinct.simps(2) drop0 drop_Suc_Cons in_set_dropD notin_List_update)
-   apply(rule conjI)
-    apply(metis Int_iff List_def List_distinct Path.simps(2) Suc_le_length_iff addr.simps distinct.simps(2) distinct_length_2_or_more empty_iff notin_List_update)
-   apply(rule conjI)
-    apply(smt (verit) List_def Path.simps Suc_le_length_iff addr.simps fun_upd_other fun_upd_same insert_iff list.set(2) splice.simps(2) splice_Nil2 take0 take_Suc_Cons)
-   apply(smt (verit) List_def List_distinct Path.simps(2) Suc_le_length_iff addr.simps distinct.simps(2) drop0 drop_Suc_Cons in_set_dropD notin_List_update)
-  apply(simp add: test2)
-  apply(rule conjI)
-   apply(subgoal_tac "List tl (tl y) (drop (Suc n) Qs)")
-  using notin_List_update
-    apply(metis Cons_nth_drop_Suc List_def List_hd_not_in_tl Path.simps(2) addr.simps disjoint_iff drop_all in_set_dropD le_neq_implies_less le_trans list.set_intros(1))
-   apply(metis drop_Suc list.sel(3) tl_drop)
-  apply(rule conjI)
-   apply(metis drop_all leI le_less_Suc_eq list.discI)
-  (* final case *)
-  apply(case_tac "drop n Ps")
-   apply(simp)
-  apply(subgoal_tac "splice (take (Suc n) Ps) (take (Suc n) Qs)
-                   = splice (take n Ps) (take n Qs) @ [a,y]")
-   defer
-   apply(simp add: splice2)
-  apply(clarsimp)
-  apply(thin_tac "splice (take (Suc n) Ps) (take (Suc n) Qs)
-                = splice (take n Ps) (take n Qs) @ [a, y]")
-  apply(rule conjI)
-   defer
-   apply(metis Int_iff empty_iff fun_upd_same fun_upd_twist in_set_dropD list.set_intros(1))
-  apply(subgoal_tac "a \<notin> set (take n Qs) \<and> y \<notin> set (take n Ps) \<and>
+    defer
+    apply(rule conjI)
+     apply (smt (verit, ccfv_SIG) Cons_nth_drop_Suc List_def List_hd_not_in_tl Path.simps(2) addr.simps append_take_drop_id disjoint_iff le_neq_implies_less le_trans list.sel(3) list.set_intros(1) not_distinct_conv_prefix notin_List_update set_drop_subset subset_code(1) take_all)
+    apply(rule conjI)
+     apply (metis drop_all list.discI not_less_eq_eq)
+    apply(rule conjI)
+     prefer 3
+     apply(clarsimp)
+     apply (metis List_app splice1)
+    apply(case_tac "drop n Ps")
+     apply (metis drop_eq_Nil le_trans list.discI)
+    apply(clarsimp simp add: splice2)
+    apply(subgoal_tac "a \<notin> set (take n Qs) \<and> y \<notin> set (take n Ps) \<and>
                      a \<notin> set (take n Ps) \<and> y \<notin> set (take n Qs)")
-   apply(simp add: splice_set)
-  apply(metis append_take_drop_id disjoint_iff distinct_take in_set_dropD in_set_takeD list.set_intros(1) not_distinct_conv_prefix)
+     apply(simp add: splice_set)
+    apply (metis Int_iff append_take_drop_id distinct_take empty_iff in_set_conv_decomp in_set_takeD not_distinct_conv_prefix)
+   apply (smt (verit, del_insts) Cons_nth_drop_Suc List_def List_distinct Path.simps(2) addr.simps append_take_drop_id disjoint_iff distinct.simps(2) le_neq_implies_less le_trans list.set_intros(1) not_distinct_conv_prefix notin_List_update set_drop_subset subset_code(1) take_all)+
   done
 
-(* unused
-lemma Path_app:
-  "\<And>tl. Path tl p la pp \<Longrightarrow> Path tl pp lb ppp
-     \<Longrightarrow> Path tl p (la @ lb) ppp"
-  apply(induct la arbitrary: p)
-  by auto
-*)
+lemma "VARS tl p q pp qq
+  {List tl p Ps \<and> List tl q Qs \<and> set Ps \<inter> set Qs = {} \<and> size Qs \<le> size Ps}
+  pp := p;
+  WHILE q \<noteq> Null
+  INV {\<exists>as bs qs.
+    distinct as \<and> Path tl p as pp \<and> List tl pp bs \<and> List tl q qs \<and>
+    set bs \<inter> set qs = {} \<and> set as \<inter> (set bs \<union> set qs) = {} \<and>
+    size qs \<le> size bs \<and> splice Ps Qs = as @ splice bs qs}
+  DO qq := q^.tl; q^.tl := pp^.tl; pp^.tl := q; pp := q^.tl; q := qq OD
+  {List tl p (splice Ps Qs)}"
+  apply (vcg)
+    apply simp_all
+    apply(rule_tac x = "[]" in exI)
+    apply fastforce
+   apply clarsimp
+   apply(rename_tac y bs qqs)
+   apply(case_tac bs;clarsimp)
+   apply(rename_tac x bbs)
+   apply(rule_tac x = "as @ [x,y]" in exI)
+   apply simp
+   apply(rule_tac x = "bbs" in exI)
+   apply simp
+   apply(rule_tac x = "qqs" in exI)
+   apply simp
+  apply (auto simp: List_app)
+  done
+
 end
